theories/InstantiationStlcInstances.v
@@ -1,0 +1,48 @@
+(******************************************************************************)
+(* Copyright (c) 2023 Denis Carnier, Steven Keuchel                           *)
+(* All rights reserved.                                                       *)
+(*                                                                            *)
+(* Redistribution and use in source and binary forms, with or without         *)
+(* modification, are permitted provided that the following conditions are     *)
+(* met:                                                                       *)
+(*                                                                            *)
+(* 1. Redistributions of source code must retain the above copyright notice,  *)
+(*    this list of conditions and the following disclaimer.                   *)
+(*                                                                            *)
+(* 2. Redistributions in binary form must reproduce the above copyright       *)
+(*    notice, this list of conditions and the following disclaimer in the     *)
+(*    documentation and/or other materials provided with the distribution.    *)
+(*                                                                            *)
+(* THIS SOFTWARE IS PROVIDED BY THE COPYRIGHT HOLDERS AND CONTRIBUTORS        *)
+(* "AS IS" AND ANY EXPRESS OR IMPLIED WARRANTIES, INCLUDING, BUT NOT LIMITED  *)
+(* TO, THE IMPLIED WARRANTIES OF MERCHANTABILITY AND FITNESS FOR A PARTICULAR *)
+(* PURPOSE ARE DISCLAIMED. IN NO EVENT SHALL THE COPYRIGHT HOLDER OR          *)
+(* CONTRIBUTORS BE LIABLE FOR ANY DIRECT, INDIRECT, INCIDENTAL, SPECIAL,      *)
+(* EXEMPLARY, OR CONSEQUENTIAL DAMAGES (INCLUDING, BUT NOT LIMITED TO,        *)
+(* PROCUREMENT OF SUBSTITUTE GOODS OR SERVICES; LOSS OF USE, DATA, OR         *)
+(* PROFITS; OR BUSINESS INTERRUPTION) HOWEVER CAUSED AND ON ANY THEORY OF     *)
+(* LIABILITY, WHETHER IN CONTRACT, STRICT LIABILITY, OR TORT (INCLUDING       *)
+(* NEGLIGENCE OR OTHERWISE) ARISING IN ANY WAY OUT OF THE USE OF THIS         *)
+(* SOFTWARE, EVEN IF ADVISED OF THE POSSIBILITY OF SUCH DAMAGE.               *)
+(******************************************************************************)
+
+#[export] Instance lift_ty : Lift OTy Ty :=
+  fix lift_ty (t : Ty) w : OTy w :=
+    match t with
+    | ty.bool       => oty.bool
+    | ty.func t1 t2 => oty.func (lift_ty t1 w) (lift_ty t2 w)
+    end.
+
+#[export] Instance lift_env : Lift OEnv Env :=
+  fun E w => fmap (fun t => lift (Lift := lift_ty) t) E.
+
+#[export] Instance inst_ty : Inst OTy Ty :=
+  fix inst_ty {w} t ι :=
+    match t with
+    | oty.evar αIn   => env.lookup ι αIn
+    | oty.bool       => ty.bool
+    | oty.func t1 t2 => ty.func (inst_ty t1 ι) (inst_ty t2 ι)
+    end.
+
+#[export] Instance inst_env : Inst OEnv Env :=
+  fun w Γ ι => base.fmap (fun t : OTy w => inst t ι) Γ.
